fix Multiplication

code/experimental/rsa/Multiplication.fst
@@ -9,40 +9,36 @@ module U64 = FStar.UInt64
 
 type bignum = buffer FStar.UInt64.t
 
+type lbignum (len:U32.t) = 
+     b:bignum{length b = U32.v len} 
+
+type bnlen = (l:U32.t{U32.v l > 0 /\ U32.v l <= 8192})
+
 val mult64: x:U64.t -> y:U64.t -> Tot (U64.t * U64.t)
 #set-options "--z3rlimit 300"
 let mult64 x y =
     let a = U64.(x >>^ 32ul) in
-    assert(U64.v a < pow2 32);
     let b = uint64_to_uint32 x in let b = uint32_to_uint64 b in
-    assert(U64.v b < pow2 32);
     let c = U64.(y >>^ 32ul) in
-    assert(U64.v c < pow2 32);
-    let d = uint64_to_uint32 x in let d = uint32_to_uint64 d in
-    assert(U64.v d < pow2 32);
+    let d = uint64_to_uint32 y in let d = uint32_to_uint64 d in
 
-    let ac = U64.(a *^ c) in
-    let bc = U64.(b *^ c) in
-    let ad = U64.(a *^ d) in
-    let bd = U64.(b *^ d) in
+    let ac = U64.(a *%^ c) in
+    let bc = U64.(b *%^ c) in
+    let ad = U64.(a *%^ d) in
+    let bd = U64.(b *%^ d) in
 
     let t1 = U64.(bd >>^ 32ul) in
-    //assert(U64.v t1 < pow2 32);
     let t2 = uint64_to_uint32 bc in let t2 = uint32_to_uint64 t2 in
-    //assert(U64.v t2 < pow2 32);
     let t3 = uint64_to_uint32 ad in let t3 = uint32_to_uint64 t3 in 
-    //assert(U64.v t3 < pow2 32);
     let mid = U64.(t1 +%^ t2 +%^ t3) in
 
     let t1 = U64.(bc >>^ 32ul) in
-    //assert(U64.v t1 < pow2 32);
-    let t2 = U64.(mid >>^ 32ul) in
-    //assert(U64.v t2 < pow2 32);
-    
-    let upper64 = U64.(ac +%^ t1 +%^ t2) in
-    let t3 = uint64_to_uint32 bd in let t3 = uint32_to_uint64 t3 in
-    //assert(U64.v t3 < pow2 32); 
-    let lower64 = U64.((mid <<^ 32ul) |^ t3) in
+    let t2 = U64.(ad >>^ 32ul) in
+    let t3 = U64.(mid >>^ 32ul) in
+
+    let upper64 = U64.(ac +%^ t1 +%^ t2 +%^ t3) in
+    let t4 = uint64_to_uint32 bd in let t4 = uint32_to_uint64 t4 in
+    let lower64 = U64.((mid <<^ 32ul) |^ t4) in
     (upper64, lower64)
 
 val add64: x:U64.t -> y:U64.t -> Tot (U64.t * U64.t)
@@ -52,59 +48,65 @@ let add64 x y =
     (carry, res)
 
 val mult_inner_loop:
-    aLen:U32.t ->
-    a:bignum{U32.v aLen = length a} ->
-    b:bignum ->
-    i:U32.t{U32.v i < length b} -> 
+    aLen:bnlen -> bLen:bnlen ->
+    a:lbignum aLen ->
+    b:lbignum bLen ->
+    i:U32.t{U32.v i < U32.v bLen} ->
     j:U32.t{U32.v j <= U32.v aLen} ->
-    carry:U64.t -> 
-    res:bignum{U32.v i + U32.v j < length res /\ length res = U32.v aLen + length b} -> Stack unit
+    carry:U64.t ->
+    res:lbignum U32.(aLen +^ bLen) -> Stack unit
     (requires (fun h -> live h a /\ live h b /\ live h res))
     (ensures  (fun h0 _ h1 -> live h0 a /\ live h0 b /\ live h0 res /\ 
         live h1 a /\ live h1 b /\ live h1 res /\ modifies_1 res h0 h1))
-let rec mult_inner_loop aLen a b i j carry res =
-    if U32.(j <^ aLen) then
-       (let (carry1, s1) = mult64 a.(j) b.(i) in
+
+let rec mult_inner_loop aLen bLen a b i j carry res =
+    if U32.(j <^ aLen) then begin
+        let (carry1, s1) = mult64 a.(j) b.(i) in
         let (carry2, s2) = add64 res.(U32.(i +^ j)) s1 in
         let (carry3, s3) = add64 s2 carry in
         let carry = U64.(carry1 +%^ carry2 +%^ carry3) in
         res.(U32.(i +^ j)) <- s3;
-        mult_inner_loop aLen a b i U32.(j +^ 1ul) carry res)
-    else res.(U32.(i +^ aLen)) <- carry
+        mult_inner_loop aLen bLen a b i U32.(j +^ 1ul) carry res
+        end
+    else 
+        res.(U32.(i +^ aLen)) <- carry
 
 val mult_outer_loop:
-    aLen:U32.t -> bLen:U32.t ->
-    a:bignum{U32.v aLen = length a} -> 
-    b:bignum{U32.v bLen = length b} ->
-    i:U32.t{U32.(i <=^ bLen)} -> 
-    res:bignum{U32.v aLen + U32.v bLen = length res} -> Stack unit
+    aLen:bnlen -> bLen:bnlen ->
+    a:lbignum aLen ->
+    b:lbignum bLen ->
+    i:U32.t{U32.v i <= U32.v bLen} ->
+    res:lbignum U32.(aLen +^ bLen) -> Stack unit
     (requires (fun h -> live h a /\ live h b /\ live h res))
     (ensures  (fun h0 _ h1 -> live h0 a /\ live h0 b /\ live h0 res /\
         live h1 a /\ live h1 b /\ live h1 res /\ modifies_1 res h0 h1))
+
 let rec mult_outer_loop aLen bLen a b i res =
-    if U32.(i <^ bLen) then
-       (mult_inner_loop aLen a b i 0ul 0uL res;
-        mult_outer_loop aLen bLen a b U32.(i +^ 1ul) res)
-    else ()
+    if U32.(i <^ bLen) then begin
+        mult_inner_loop aLen bLen a b i 0ul 0uL res;
+        mult_outer_loop aLen bLen a b U32.(i +^ 1ul) res
+        end
 
 (* res = a * b *)
 val mult:
-    aLen:U32.t -> bLen:U32.t ->
-    a:bignum{U32.v aLen = length a} -> 
-    b:bignum{U32.v bLen = length b} ->
-    res:bignum{U32.v aLen + U32.v bLen = length res} -> Stack unit
+    aLen:bnlen -> bLen:bnlen ->
+    a:lbignum aLen ->
+    b:lbignum bLen ->
+    res:lbignum U32.(aLen +^ bLen) -> Stack unit
     (requires (fun h -> live h a /\ live h b /\ live h res))
     (ensures  (fun h0 _ h1 -> live h0 a /\ live h0 b /\ live h0 res /\
         live h1 a /\ live h1 b /\ live h1 res /\ modifies_1 res h0 h1))
+        
 let mult aLen bLen a b res =
     mult_outer_loop aLen bLen a b 0ul res
 
 (* TODO: res = a * a *)
 val sqr:
-    aLen:U32.t -> a:bignum{U32.v aLen = length a} ->
-    res:bignum{length res = U32.v aLen + U32.v aLen} -> Stack unit
+    aLen:bnlen -> a:lbignum aLen ->
+    res:lbignum U32.(aLen +^ aLen) -> Stack unit
     (requires (fun h -> live h a /\ live h res))
     (ensures  (fun h0 _ h1 -> live h0 a /\ live h0 res /\ 
-        live h1 res /\ modifies_1 res h0 h1))
+        live h1 a /\ live h1 res /\ modifies_1 res h0 h1))
+        
 let sqr aLen a res =
     mult aLen aLen a a res
